@prefix adrf: <https://github.com/Coleridge-Initiative/adrf-onto/wiki/Vocabulary#> .

## Referenced Namespaces

@prefix dbo:    <http://dbpedia.org/ontology/> .
@prefix dbr:	<http://dbpedia.org/resource/> .
@prefix dct:	<http://purl.org/dc/elements/1.1/#> .
@prefix foaf:	<http://xmlns.com/foaf/0.1/> .
@prefix madsrdf: <http://www.loc.gov/mads/rdf/v1#> .
@prefix owl:	<http://www.w3.org/2002/07/owl#> .
@prefix rdf:	<http://www.w3.org/1999/02/22-rdf-syntax-ns#> .
@prefix rdfs:	<http://www.w3.org/2000/01/rdf-schema#> .
@prefix schema:	<http://schema.org/> .
@prefix skos:	<http://www.w3.org/2004/02/skos/core#> .
@prefix void: <http://rdfs.org/ns/void#> .
@prefix wn:	<http://www.ontologyportal.org/WordNet.owl#> .
@prefix xml:	<http://www.w3.org/XML/1998/namespace> .
@prefix xsd:	<http://www.w3.org/2001/XMLSchema#> .


adrf:ADRF_Ontology rdf:type skos:ConceptScheme;
  skos:definition "A mid-level ontology for linked data within the ADRF framework use cases"@en;
  skos:prefLabel "ADRF Ontology"@en;
  .

adrf:Topic a madsrdf:Topic;
  skos:definition "Concepts tied to LOC upper ontology http://id.loc.gov/authorities/subjects.html"@en;
  skos:topConceptOf adrf:ADRF_Ontology;
  a madsrdf:Authority;
  .

## Local Entities

adrf:Dataset a skos:Concept;
  skos:definition "A collection of tables and metadata, managed by a responsible party"@en;
  skos:topConceptOf adrf:ADRF_Ontology;
  skos:prefLabel "dataset"@en;
  madsrdf:hasRelatedAuthority <http://id.loc.gov/authorities/subjects/sh2018002256>;
  owl:sameAs schema:Dataset;
  owl:sameAs dbr:Data_set;
  .

#  skos:broader adrf:Linked_Data.
