@prefix adrf: <https://github.com/DerwenAI/adrf-onto/wiki/Vocabulary#> .

@prefix dbr: <http://dbpedia.org/page/> .
@prefix dct: <http://purl.org/dc/elements/1.1/#> .
@prefix madsrdf: <http://www.loc.gov/mads/rdf/v1#>.
@prefix owl: <http://www.w3.org/2002/07/owl#> .
@prefix rdf: <http://www.w3.org/1999/02/22-rdf-syntax-ns#> .
@prefix rdfs: <http://www.w3.org/2000/01/rdf-schema#> .
@prefix schema: <http://schema.org/>.
@prefix skos: <http://www.w3.org/2004/02/skos/core#> .
@prefix wn: <http://www.ontologyportal.org/WordNet.owl#> .
@prefix xml: <http://www.w3.org/XML/1998/namespace> .
@prefix xsd: <http://www.w3.org/2001/XMLSchema#> .


adrf:ADRF_Ontology rdf:type skos:ConceptScheme;
  skos:prefLabel "ADRF Ontology"@en;
  skos:definition "A mid-level ontology for linked data within ADRF framework use cases"@en.

adrf:Topic a madsrdf:Topic;
  a madsrdf:Authority;
  skos:topConceptOf adrf:ADRF_Ontology;
  skos:definition "Concepts tied to LOC upper ontology http://id.loc.gov/authorities/subjects.html"@en.


## Entity Types

adrf:Dataset a skos:Concept;
  owl:sameAs schema:Dataset;
  owl:sameAs dbr:Data_set;
  madsrdf:hasRelatedAuthority <http://id.loc.gov/authorities/subjects/sh2018002256>;
  skos:topConceptOf adrf:ADRF_Ontology;
  skos:prefLabel "dataset"@en;
  skos:definition "A collection of tables and metadata, managed by a responsible party"@en.

#  skos:broader adrf:Linked_Data.
