@base <https://github.com/Coleridge-Initiative/adrf-onto/wiki/Vocabulary> .

@prefix cito:	<http://purl.org/spar/cito/> .
@prefix dbo:    <http://dbpedia.org/ontology/> .
@prefix dbr:	<http://dbpedia.org/resource/> .
@prefix dcat:	<http://www.w3.org/ns/dcat#> .
@prefix dct:	<http://purl.org/dc/terms/> .
@prefix dcterms: <http://purl.org/dc/terms/> .
@prefix dctypes: <http://purl.org/dc/dcmitype/> .
@prefix fabio:	<http://purl.org/spar/fabio/> .
@prefix foaf:	<http://xmlns.com/foaf/0.1/> .
@prefix madsrdf: <http://www.loc.gov/mads/rdf/v1#> .
@prefix owl:	<http://www.w3.org/2002/07/owl#> .
@prefix pav:	<http://purl.org/pav/> .
@prefix prism:	<http://prismstandard.org/namespaces/basic/2.0/> .
@prefix rdf:	<http://www.w3.org/1999/02/22-rdf-syntax-ns#> .
@prefix rdfs:	<http://www.w3.org/2000/01/rdf-schema#> .
@prefix schema:	<http://schema.org/> .
@prefix skos:	<http://www.w3.org/2004/02/skos/core#> .
@prefix void:	<http://rdfs.org/ns/void#> .
@prefix wn:	<http://www.ontologyportal.org/WordNet.owl#> .
@prefix xml:	<http://www.w3.org/XML/1998/namespace> .
@prefix xsd:	<http://www.w3.org/2001/XMLSchema#> .


:ADRF_Ontology rdf:type skos:ConceptScheme ;
  skos:definition "A mid-level ontology for linked data within the ADRF framework use cases"@en ;
  skos:prefLabel "ADRF Ontology"@en ;
  .

:Catalog a dcat:Catalog ;
  skos:topConceptOf :ADRF_Ontology ;
  dct:title "ADRF Data Catalog" ;
  rdfs:label "ADRF Data Catalog" ;
  foaf:homepage <https://coleridgeinitiative.org/> ;
  dct:language <http://id.loc.gov/vocabulary/iso639-1/en>  ;
  .

:Topic a madsrdf:Topic ;
  skos:definition "Concepts tied to LOC upper ontology http://id.loc.gov/authorities/subjects.html"@en ;
  skos:topConceptOf :ADRF_Ontology ;
  a madsrdf:Authority ;
  .

:Dataset a dcat:Dataset ;
  skos:definition "A collection of tables and metadata used within the ADRF framework, managed by a responsible party"@en ;
  skos:topConceptOf :ADRF_Ontology ;
  skos:prefLabel "dataset"@en ;
  madsrdf:hasRelatedAuthority <http://id.loc.gov/authorities/subjects/sh2018002256> ;
  owl:sameAs dbr:Data_set ;
  .

:Researcher a foaf:Person ;
  skos:definition "An author of a research publication that uses datasets for research"@en ;
  skos:topConceptOf :ADRF_Ontology ;
  skos:prefLabel "author"@en ;
  madsrdf:hasRelatedAuthority <http://id.loc.gov/authorities/subjects/sh85089630> ;
  owl:sameAs dbr:Author ;
  .

:ResearchPublication a fabio:ResearchPaper ;
  skos:definition "A research publication that uses datasets for research"@en ;
  skos:topConceptOf :ADRF_Ontology ;
  skos:prefLabel "research publication"@en ;
  madsrdf:hasRelatedAuthority <http://id.loc.gov/authorities/subjects/sh2004003366> ;
  owl:sameAs dbr:Publication ;
  .

:DatasetProvider a foaf:Organization ;
  skos:definition "An organizaiton that publishes and curates research datasets"@en ;
  skos:topConceptOf :ADRF_Ontology ;
  skos:prefLabel "dataset provider"@en ;
  madsrdf:hasRelatedAuthority <http://id.loc.gov/authorities/subjects/sh85066157> ;
  owl:sameAs dbr:Data_publishing ;
  .


:Corpus a skos:Collection ;
  dct:title "ADRF Corpus of research publications" ;
  rdfs:label "ADRF Corpus" ;
  .

:publication a rdf:Property, owl:ObjectProperty ;
  rdfs:label "publication"@en ;
  rdfs:subPropertyOf dct:hasPart ;
  rdfs:domain :Corpus ;
  rdfs:range :ResearchPublication ;
  .
